gravy/src/org/gravy/checker/AbstractChecker.java
@@ -39,23 +39,7 @@ public abstract class AbstractChecker implements Runnable {
 		
 	protected HashSet<BasicBlock> feasibleBlocks = new HashSet<BasicBlock>();
 	protected HashSet<BasicBlock> infeasibleBlocks = new HashSet<BasicBlock>();
-	protected HashSet<BasicBlock> infeasibleBlocksUnderPost = new HashSet<BasicBlock>();
-
-	//TODO: this is a very trivial way of reporting
-	public long countFeasibleBlock() {
-		return feasibleBlocks.size();
-	}
-
-	//TODO: this is a very trivial way of reporting
-	public long countInfeasibleBlock() {
-		return infeasibleBlocks.size();
-	}
-
-	//TODO: this is a very trivial way of reporting
-	public long countInfeasibleBlockUnderPost() {
-		return infeasibleBlocksUnderPost.size();
-	}
-	
+	protected HashSet<BasicBlock> infeasibleBlocksUnderPost = new HashSet<BasicBlock>();	
 	
 	protected Prover prover = null;
 	
@@ -89,7 +73,6 @@ public abstract class AbstractChecker implements Runnable {
 	public void shutDownProver() {
 		if (null == this.prover)
 			return;
-
 		this.prover.shutdown();
 		this.prover = null;	
 	}
